refine memcpy + realloc
realloc was not allocating given a null ptr,
maybe segfaults will vanish?

src/StarMalloc.fst
@@ -70,46 +70,112 @@ let getsize (ptr: array U8.t)
     return s1
   )
 
-
 assume
 val memcpy_u8 (dest src: array U8.t) (n: US.t)
-  : SteelT (array U8.t)
+  : Steel (array U8.t)
   (A.varray dest `star` A.varray src)
   (fun _ -> A.varray dest `star` A.varray src)
-
-
+  (requires fun _ ->
+    A.length dest >= US.v n /\
+    A.length src >= US.v n
+  )
+  (ensures fun h0 r h1 ->
+    A.length dest >= US.v n /\
+    A.length src >= US.v n /\
+    Seq.slice (A.asel dest h1) 0 (US.v n)
+    ==
+    Seq.slice (A.asel src h0) 0 (US.v n) /\
+    A.asel src h1 == A.asel src h0
+  )
 
 module G = FStar.Ghost
 
+let realloc_vp (status: nat{status < 3})
+  (ptr: array U8.t)
+  (new_ptr: array U8.t)
+  (r: array U8.t)
+  : vprop
+  = match status with
+  // success
+  | 0 -> null_or_varray r
+  // new allocation fails, cannot memcpy,
+  // returning previous allocation
+  | 1 -> null_or_varray ptr
+  // new_allocation succeeds, freeing old allocation fails
+  // returning null
+  | 2 -> null_or_varray ptr `star` null_or_varray new_ptr
+
+#restart-solver
+
+#push-options "--z3rlimit 100 --compat_pre_typed_indexed_effects"
 let realloc (ptr: array U8.t) (new_size: US.t)
-  : Steel (G.erased bool & array U8.t)
-  (A.varray ptr)
-  (fun r -> A.varray (snd r))
+  : Steel (array U8.t & (G.erased (x:nat{x < 3}) & G.erased (array U8.t)))
+  (null_or_varray ptr)
+  (fun r -> realloc_vp (G.reveal (fst (snd r))) ptr (snd (snd r)) (fst r))
   (requires fun _ -> A.is_full_array ptr)
-  (ensures fun _ _ _ -> True)
+  (ensures fun _ r _ ->
+    not (A.is_null (fst r)) ==> A.length (fst r) >= US.v new_size
+  )
   =
-  let old_size = getsize ptr in
-  if old_size = 0sz then (
-    sladmit ();
-    return (G.hide false, A.null #U8.t)
+  if A.is_null ptr then (
+    // In case that ptr is a null pointer, the function behaves
+    // like malloc, assigning a new block of size bytes and
+    // returning a pointer to its beginning.
+    change_equal_slprop (null_or_varray ptr) emp;
+    let new_ptr = malloc new_size in
+    change_equal_slprop
+      (if A.is_null new_ptr then emp else A.varray new_ptr)
+      (realloc_vp 0 (A.null #U8.t) (A.null #U8.t) new_ptr);
+    return (new_ptr, (G.hide 0, G.hide (A.null #U8.t)))
   ) else (
+    change_equal_slprop (null_or_varray ptr) (A.varray ptr);
     let new_ptr = malloc new_size in
     if (A.is_null new_ptr) then (
-      sladmit ();
-      return (G.hide false, A.null #U8.t)
+      // If the function fails to allocate the requested block
+      // of memory, a null pointer is returned, and the memory
+      // block pointed to by argument ptr is not deallocated
+      // (it is still valid, and with its contents unchanged).
+      change_equal_slprop
+        (if A.is_null new_ptr then emp else A.varray new_ptr)
+        emp;
+      change_equal_slprop
+        (A.varray ptr)
+        (realloc_vp 1 ptr (A.null #U8.t) (A.null #U8.t));
+      return (A.null #U8.t, (G.hide 1, G.hide (A.null #U8.t)))
     ) else (
+      // The content of the memory block is preserved up to the
+      // lesser of the new and old sizes, even if the block is
+      // moved to a new location. If the new size is larger, the
+      // value of the newly allocated portion is indeterminate.
       change_equal_slprop
         (if A.is_null new_ptr then emp else A.varray new_ptr)
         (A.varray new_ptr);
-      let new_size  = if US.lte new_size old_size then new_size else old_size in
-      let _ = memcpy_u8 new_ptr ptr new_size in
+      let old_size = getsize ptr in
+      assume (US.v old_size == A.length ptr);
+      assert (A.length new_ptr >= US.v new_size);
+      let min_of_sizes =
+        if US.lte new_size old_size
+        then new_size
+        else old_size in
+      let _ = memcpy_u8 new_ptr ptr min_of_sizes in
+      change_equal_slprop
+        (A.varray new_ptr)
+        (null_or_varray new_ptr);
       let b = free ptr in
       if b then (
-        sladmit ();
-        return (G.hide true, new_ptr)
+        change_equal_slprop
+          (if b then emp else A.varray ptr) emp;
+        change_equal_slprop
+          (null_or_varray new_ptr)
+          (realloc_vp 0 ptr (A.null #U8.t) new_ptr);
+        return (new_ptr, (G.hide 0, G.hide (A.null #U8.t)))
       ) else (
-        sladmit ();
-        return (G.hide false, A.null #U8.t)
+        change_equal_slprop
+          (if b then emp else A.varray ptr) (null_or_varray ptr);
+        change_equal_slprop
+          (null_or_varray ptr `star` null_or_varray new_ptr)
+          (realloc_vp 2 ptr new_ptr (A.null #U8.t));
+        return (A.null #U8.t, (G.hide 2, G.hide new_ptr))
       )
     )
   )
